Lampe/Tests/Errors.lean
@@ -1,0 +1,71 @@
+import Lampe
+
+open Lampe
+
+noir_def hello<>() -> String<5 : u32> := {
+  "hello"
+}
+
+def helloEnv : Env := .mk [hello] []
+ /- testing enter_decl error reporting -/
+
+/--
+error: Unable to find a declaration in the environment with the right name
+-/
+#guard_msgs in
+theorem enter_decl_error : STHoare p env ⟦⟧ (hello.call h![] h![])
+    fun output => (String.mk output.toList) = "hello" := by
+  enter_decl
+
+/- testing enter_block_as error reporting -/
+
+/--
+error: failed to synthesize
+  OfNat String 5
+numerals are polymorphic in Lean, but the numeral `5` cannot be used in a context where the expected type is
+  String
+due to the absence of the instance above
+
+Additional diagnostic information may be available using the `set_option diagnostics true` command.-/
+#guard_msgs in
+theorem enter_block_error : STHoare p helloEnv ⟦⟧ (hello.call h![] h![])
+    fun output => (String.mk output.toList) = "hello" := by
+  enter_decl
+  step_as (⟦⟧) (fun (v : Tp.denote p (Tp.str 5)) => (String.mk v.toList) = 5)
+  sorry
+
+/- testing steps error messaging -/
+
+/-- error: unknown identifier 'bad_lemma'-/
+#guard_msgs in
+theorem steps_error : STHoare p helloEnv ⟦⟧ (hello.call h![] h![])
+    fun output => (String.mk output.toList) = "hello" := by
+  enter_decl
+  steps [bad_lemma]
+  sorry
+
+noir_def loop_fn<>() -> Field := {
+  let mut (t : Field) = 1 : Field;
+
+  for _i in (0 : u32)..(5 : u32) do {
+    t = (#_fMul returning Field)(t, 2 : Field);
+  } ;
+  t
+}
+
+def loopEnv : Env := .mk [loop_fn] []
+
+/- testing loop_inv error reporting -/
+
+/--
+error: unknown identifier 'u'
+---
+error: final singleton is not equal
+-/
+#guard_msgs in
+theorem loop_inv_error : STHoare p loopEnv ⟦⟧ (loop_fn.call h![] h![])
+    fun output => output = (32 : Tp.denote p Tp.field) := by
+  enter_decl
+  steps
+  loop_inv fun i _ _ => [u ↦ ⟨Tp.field, 3⟩] -- random mal-formed loop invariant to show it works
+  all_goals sorry
